theories/CScoping.v
@@ -19,16 +19,6 @@ Inductive ccscoping (Γ : cscope) : cterm → cmode → Prop :=
       nth_error Γ x = Some (Some m) →
       ccscoping Γ (cvar x) m
 
-| cscope_close :
-    ∀ m t,
-      ccscoping (None :: Γ) t m →
-      ccscoping Γ (close t) m
-
-| cscope_Close :
-    ∀ m A,
-      ccscoping (None :: Γ) A m →
-      ccscoping Γ (Close A) m
-
 | scpoe_sort :
     ∀ m i,
       ccscoping Γ (cSort m i) cType
