theories/CTyping.v
@@ -47,16 +47,6 @@ Inductive conversion (Γ : ccontext) : cterm → cterm → Prop :=
     ∀ i j,
       Γ ⊢ᶜ cSort cProp i ≡ cSort cProp j
 
-| cong_close :
-    ∀ u v,
-      None :: Γ ⊢ᶜ u ≡ v →
-      Γ ⊢ᶜ close u ≡ close v
-
-| cong_Close :
-    ∀ A B,
-      None :: Γ ⊢ᶜ A ≡ B →
-      Γ ⊢ᶜ Close A ≡ Close B
-
 | ccong_Pi :
     ∀ mx A A' B B',
       Γ ⊢ᶜ A ≡ A' →
@@ -116,16 +106,6 @@ Inductive ctyping (Γ : ccontext) : cterm → cterm → Prop :=
     ∀ x m A,
       nth_error Γ x = Some (Some (m, A)) →
       Γ ⊢ᶜ cvar x : (plus (S x)) ⋅ A
-
-| ctype_close :
-    ∀ t A,
-      None :: Γ ⊢ᶜ t : A →
-      Γ ⊢ᶜ close t : Close A
-
-| ctype_Close :
-    ∀ A m i,
-      None :: Γ ⊢ᶜ A : cSort m i →
-      Γ ⊢ᶜ Close A : cSort m i
 
 | ctype_sort :
     ∀ m i,
