theories/Erasure.v
@@ -67,7 +67,7 @@ Equations erase_term (Γ : scope) (t : term) : cterm := {
     if relm mx && negb (isProp m)
     then ctyval (cPi cType ⟦ Γ | A ⟧τ ⟦ mx :: Γ | B ⟧τ) (clam cType ⟦ Γ | A ⟧τ ⟦ mx :: Γ | B ⟧∅)
     else if isGhost m && isGhost mx
-    then ctyval (⟦ Γ | A ⟧τ ⇒[ cType ] (Close ⟦ mx :: Γ | B ⟧τ)) (clam cType ⟦ Γ | A ⟧τ (S ⋅ close ⟦ mx :: Γ | B ⟧∅))
+    then ctyval (⟦ Γ | A ⟧τ ⇒[ cType ] (close ⟦ mx :: Γ | B ⟧τ)) (clam cType ⟦ Γ | A ⟧τ (S ⋅ close ⟦ mx :: Γ | B ⟧∅))
     else if isProp m
     then ctt
     else close ⟦ mx :: Γ | B ⟧ε ;
@@ -272,9 +272,13 @@ Proof.
     + destruct m. all: try discriminate.
       destruct mx. all: try discriminate.
       cbn in *.
+      (* TODO scoping / typing tactic that uses close rules *)
       repeat constructor. all: eauto.
-      * asimpl. unfold Ren_cterm, upRen_cterm_cterm.
-        eapply cscoping_ren. 2: eauto.
+      * asimpl. unfold Ren_cterm, upRen_cterm_cterm, Subst_cterm, VarInstance_cterm.
+        rewrite substRen_cterm. asimpl.
+
+
+        (* eapply cscoping_ren. 2: eauto.
         eapply crscoping_shift. eapply crscoping_S.
       * asimpl. unfold Ren_cterm, upRen_cterm_cterm.
         eapply cscoping_ren. 2: eauto.
@@ -300,7 +304,8 @@ Proof.
     assumption.
   - cbn - [mode_inb]. destruct_if e. 2: discriminate.
     constructor. eauto.
-Qed.
+Qed. *)
+Admitted.
 
 (** Erasure commutes with renaming **)
 
@@ -360,7 +365,7 @@ Proof.
     2:{ eapply rscoping_upren. eassumption. }
     2:{ eapply rscoping_comp_upren. assumption. }
     destruct_ifs. all: try solve [ eauto ].
-    asimpl. repeat unfold_funcomp.
+    (* asimpl. repeat unfold_funcomp.
     unfold Ren_cterm, upRen_cterm_cterm. asimpl. repeat unfold_funcomp.
     cbn. unfold upRen_cterm_cterm. unfold up_ren.
     asimpl. repeat unfold_funcomp.
@@ -383,7 +388,8 @@ Proof.
   - cbn - [mode_inb].
     erewrite IHt1. 2,3: eassumption.
     destruct_ifs. all: eauto.
-Qed.
+Qed. *)
+Admitted.
 
 Lemma nth_skipn :
   ∀ A (l : list A) x y d,
@@ -678,19 +684,6 @@ Proof.
   - constructor.
   - econstructor.
 Qed.
-
-(*** PROBLEM Close
-
-  Is it really a god idea? Currently close/Close is going to get in the way
-  of conversion. Like is Close (Π A B) a Π?
-  Could we have the equivalent of an application by just doing a random
-  substitution?
-  In that case, maybe close should be a definition that substitutes?
-
-  Adding computation rules is getting out of hands, it becomes harder to
-  argue that it's just to avoid technicalities.
-
-***)
 
 Theorem erase_typing :
   ∀ Γ t A,
